\documentclass{article}
\usepackage{ifthen}
\usepackage{epsfig}
\usepackage[utf8]{inputenc}
% Packages requested by user
\usepackage{amsmath}

\usepackage{newunicodechar}
  \newunicodechar{⁻}{${}^{-}$}% Superscript minus
  \newunicodechar{²}{${}^{2}$}% Superscript two
  \newunicodechar{³}{${}^{3}$}% Superscript three

\pagestyle{empty}
\begin{document}
\begin{equation*} \rho = \sqrt{ \frac{\psi - \psi_0}{\psi_1 - \psi_0} }, \end{equation*}
\pagebreak

$\psi_0$
\pagebreak

$\psi_1$
\pagebreak

$Rz$
\pagebreak

$\mathbf{B}$
\pagebreak

$B_R$
\pagebreak

$B_z$
\pagebreak

$\psi$
\pagebreak

\begin{align*} B_R &= -\frac{1}{R}\frac{\partial\psi}{\partial z}\\ B_z &= \frac{1}{R}\frac{\partial\psi}{\partial R} \end{align*}
\pagebreak

$R\phi z$
\pagebreak

$\psi(R,z)$
\pagebreak

$\phi$
\pagebreak

\begin{align*} \psi(R,Z) = &\psi_c [(1-A) (r^4/8) \\ &+ A (r^2\log(r)/2) \\ &+ c_0 \\ &+ c_1 (r^2) \\ &+ c_2 (r^2\log(r) - z^2) \\ &+ c_3 (r^4 - 4r^2z^2) \\ &+ c_4 (3r^4\log(r) - 9r^2z^2 - 12r^2\log(r)z^2 + 2z^4) \\ &+ c_5 (r^6 - 12r^4z^2 + 8r^2z^4) \\ &+ c_6 (8z^6 - 140r^2z^4 - 120r^2\log(r)z^4 + 180r^4\log(r)z^2 + 75r^4z^2 - 15r^6\log(r)) \\ &+ c_7 (z) \\ &+ c_8 (zr^2) \\ &+ c_9 (z^3 - 3zr^2\log(r)) \\ &+ c_{10} (3zr^4 - 4z^3r^2) \\ &+ c_{12} (8z^5 - 45zr^4 - 80z^3r^2\log(r) + 60zr^4\log(r)) ] \end{align*}
\pagebreak

$c_i$
\pagebreak

$A$
\pagebreak

$\psi_c$
\pagebreak

$r = R/R_0$
\pagebreak

$z = Z/R_0$
\pagebreak

\begin{equation*} B_\phi = \frac{B_0R_0}{R} \end{equation*}
\pagebreak

$N>0$
\pagebreak

\begin{equation*} \tilde{B}_\phi = B_\phi( 1 + \delta\cos(N\phi) ) \end{equation*}
\pagebreak

\begin{equation*} \delta = \delta_0 \frac{r'}{a_0}^{\alpha_0} e^{-\theta^2} \end{equation*}
\pagebreak

$\theta = \arctan(Z - z_0, R- R_0)$
\pagebreak

$r' = \sqrt{(R-R_0)^2 + (Z-Z_0)^2}$
\pagebreak

$\phi_\mathrm{max}-\phi_\mathrm{min} = 2\pi/(N+1)$
\pagebreak

$\phi_\mathrm{max}$
\pagebreak

$\phi_\mathrm{min}=0$
\pagebreak

$n_\phi = 360$
\pagebreak

$\phi_\mathrm{max}=359$
\pagebreak

$N=0$
\pagebreak

$(B_x, B_y, B_z)$
\pagebreak

$(R,z) = (0,0)$
\pagebreak

\[ \begin{bmatrix} \frac{\partial B_x}{\partial x}, &\frac{\partial B_x}{\partial y}, &\frac{\partial B_x}{\partial z} \\ \frac{\partial B_y}{\partial x}, &\frac{\partial B_y}{\partial y}, &\frac{\partial B_y}{\partial z} \\ \frac{\partial B_z}{\partial x}, &\frac{\partial B_z}{\partial y}, &\frac{\partial B_z}{\partial z} \end{bmatrix} \]
\pagebreak

$\rho$
\pagebreak

$B_phi$
\pagebreak

$ \gamma = \sqrt{\frac{1}{1-v^2/c^2}}$
\pagebreak

$v$
\pagebreak

$\gamma = \sqrt{1 + \left(\frac{p}{mc}\right)^2}$
\pagebreak

$m$
\pagebreak

$p$
\pagebreak

$\gamma = \sqrt{\frac{1 + (2\mu B/mc^2)}{1 - v_\parallel^2/c^2}}$
\pagebreak

$\mu$
\pagebreak

$v_\parallel$
\pagebreak

$B$
\pagebreak

$\gamma = \sqrt{1 + 2\mu B/mc^2 + (p_\parallel/mc)^2}$
\pagebreak

$p_\parallel$
\pagebreak

$E_\mathrm{kin}=(\gamma - 1) * m c^2$
\pagebreak

$\gamma$
\pagebreak

$\gamma = \frac{E_\mathrm{kin}}{m c^2} + 1$
\pagebreak

$E_\mathrm{kin}=(\gamma(p) - 1) * m c^2$
\pagebreak

$E_\mathrm{kin}=(\gamma(m, \mu, p_\parallel, B) - 1) * m c^2$
\pagebreak

$v = p/\gamma(p)m$
\pagebreak

$p = \gamma(v)mv$
\pagebreak

$p_\parallel = \xi p$
\pagebreak

$\xi$
\pagebreak

$\mu = (1-\xi^2)p/(2mB)$
\pagebreak

$p = \sqrt{\gamma(m,\mu,p_\parallel,B)^2 - 1} m c$
\pagebreak

$\xi = p_\parallel / p(m,\mu,p_\parallel,B) $
\pagebreak

$\rho_g = \frac{\mathbf{p}\cdot\mathbf{B}}{|q|B^2}$
\pagebreak

$q$
\pagebreak

$\mathbf{v}$
\pagebreak

$\rho_g = \frac{1}{|q|}\sqrt{\frac{2\gamma(m, \mu, p_\parallel, B) m \mu} {B}}$
\pagebreak

$\omega_g = \frac{q B}{\gamma(p) m}$
\pagebreak

$\omega_g = \frac{q B}{\gamma(m, \mu, p_\parallel, B) m}$
\pagebreak

$c_{ab} = \frac{n_b q_a^2q_b^2 \ln\Lambda_{ab}}{4\pi\epsilon_0^2}$
\pagebreak

$q_a$
\pagebreak

$q_b$
\pagebreak

$n_b$
\pagebreak

$\ln\Lambda_{ab}$
\pagebreak

$Q =-c_{ab}(q_a,q_b,n_b,\ln\Lambda_{ab})\mu_0(v_a/v_b) / (m_a m_b v_b^2)$
\pagebreak

$m_a$
\pagebreak

$m_b$
\pagebreak

$v_b$
\pagebreak

$Q'=-c_{ab}(q_a,q_b,n_b,\ln\Lambda_{ab})\mu_0'(v_a/v_b) / (m_a m_b v_b^2)$
\pagebreak

$F = -c_{ab}(q_a,q_b,n_b,\ln\Lambda_{ab})\left(m_a^{-1} + m_b^{-1}\right) \mu0(v_a/v_b) / (m_a v_b^2)$
\pagebreak

$D_\parallel=c_{ab}(q_a,q_b,n_b,\ln\Lambda_{ab})\mu_0(v_a/v_b) /(2m_a^2v_a)$
\pagebreak

$D_\parallel = 4c_{ab}(q_a,q_b,n_b,\ln\Lambda_{ab})/(6\sqrt{\pi}m_a^2vb) \;\mathrm{when}\; v_a=0$
\pagebreak

$v_a$
\pagebreak

$D_\parallel'=c_{ab}(q_a,q_b,n_b,\ln\Lambda_{ab})(\mu_0'(v_a/v_b)/v_b - \mu(v_a/v_b)/v_a)/(2m_a^2v_a)$
\pagebreak

$D_\perp=c_{ab}(q_a,q_b,n_b,\ln\Lambda_{ab})\mu_1(v_a/v_b) /(2m_a^2v_a)$
\pagebreak

$D_\perp = 4c_{ab}(q_a,q_b,n_b,\ln\Lambda_{ab})/(6\sqrt{\pi}m_a^2vb) \;\mathrm{when}\; v_a=0$
\pagebreak

$K = Q + D_\parallel' + 2D_\parallel/va$
\pagebreak

$D_parallel$
\pagebreak

$Q$
\pagebreak

$\nu = 2D_\perp/v_a^2$
\pagebreak

$D_perp$
\pagebreak

$D_X = (\frac{1}{2}(D_\parallel-D_\perp)(1-\xi^2) + D_\perp)/\omega_g^2$
\pagebreak

$xi$
\pagebreak

$D_\parallel$
\pagebreak

$\omega_g$
\pagebreak

$\mu_0(x) = (\mathrm{erf}(x) -2 x \pi^{-1/2} e^{-x^2})/x^2$
\pagebreak

$\mu_1(x) = \mathrm{erf}(x) - \frac{1}{2}\mu_0(x)$
\pagebreak

$\mu_0'(x)$
\pagebreak

\end{document}
